update npbc_array

examples/pseudo_bool/array/npbc_arrayProgScript.sml
@@ -30,6 +30,37 @@ val format_failure_def = Define`
   format_failure (lno:num) s =
   strlit "c Checking failed for top-level proof step starting at line: " ^ toString lno ^ strlit ". Reason: " ^ s ^ strlit"\n"`
 
+Definition fib_def:
+  fib n = if n ≤ (1:num) then (1:num) else fib (n-1) + fib(n-2)
+End
+
+val r = translate fib_def;
+
+val f = process_topdecs`
+  fun f x = fib x` |>append_prog;
+
+Theorem f_spec:
+  INT x xv
+  ⇒
+  app (p : 'ffi ffi_proj)
+    ^(fetch_v "f" (get_ml_prog_state()))
+    [xv]
+    (&(x ≥ 0)) (* Precondition *)
+    (POSTve
+      (λv. &(INT (&(fib (Num x))) v))
+      (λe. &F)
+    )
+Proof
+  rw[]>>
+  xcf "f" (get_ml_prog_state ())>>
+  xpull>>
+  xapp>>
+  xsimpl>>
+  fs[NUM_def,INT_def]>>
+  qexists_tac`Num x`>>simp[]>>
+  intLib.ARITH_TAC
+QED
+
 val r = translate format_failure_def;
 
 val r = translate OPTION_MAP2_DEF;
@@ -88,11 +119,8 @@ val check_cutting_arr = process_topdecs`
   | Weak c var =>
     weaken (check_cutting_arr lno fml c) var` |> append_prog
 
-Definition constraint_TYPE_def:
-  constraint_TYPE = PAIR_TYPE
-    (LIST_TYPE (PAIR_TYPE INT NUM))
-    NUM
-End
+(* Overload notation for long _TYPE relations *)
+Overload "constraint_TYPE" = ``PAIR_TYPE (LIST_TYPE (PAIR_TYPE INT NUM)) NUM``
 
 val NPBC_CHECK_CONSTR_TYPE_def = fetch "-" "NPBC_CHECK_CONSTR_TYPE_def";
 val PBC_LIT_TYPE_def = fetch "-" "PBC_LIT_TYPE_def"
@@ -143,7 +171,6 @@ Proof
     last_x_assum kall_tac>>
     every_case_tac>>fs[]>>
     xapp>>xsimpl>>
-    fs[constraint_TYPE_def]>>
     metis_tac[])
   >- ( (* Mul *)
     fs[check_cutting_list_def,NPBC_CHECK_CONSTR_TYPE_def]>>
@@ -152,7 +179,6 @@ Proof
     last_x_assum kall_tac>>
     every_case_tac>>fs[]>>
     xapp>>xsimpl>>
-    fs[constraint_TYPE_def]>>
     metis_tac[])
   >- ( (* Div *)
     fs[check_cutting_list_def,NPBC_CHECK_CONSTR_TYPE_def]>>
@@ -168,7 +194,6 @@ Proof
     asm_exists_tac>>simp[]>>
     pop_assum mp_tac>>
     TOP_CASE_TAC>>rw[]>>
-    fs[constraint_TYPE_def]>>
     metis_tac[])
   >- ( (* Sat *)
     fs[check_cutting_list_def,NPBC_CHECK_CONSTR_TYPE_def]>>
@@ -179,7 +204,6 @@ Proof
     xsimpl>>
     pop_assum mp_tac>>
     TOP_CASE_TAC>>rw[]>>
-    fs[constraint_TYPE_def]>>
     metis_tac[])
   >- ( (* Lit *)
     fs[check_cutting_list_def,NPBC_CHECK_CONSTR_TYPE_def]>>
@@ -188,7 +212,7 @@ Proof
     fs[PBC_LIT_TYPE_def]>>xmatch>>
     rpt xlet_autop>>
     xcon>>xsimpl>>
-    simp[constraint_TYPE_def,LIST_TYPE_def,PAIR_TYPE_def])
+    simp[LIST_TYPE_def,PAIR_TYPE_def])
   >> ( (* Weak *)
     fs[check_cutting_list_def,NPBC_CHECK_CONSTR_TYPE_def]>>
     xmatch>>
@@ -198,7 +222,7 @@ Proof
     xsimpl>>
     pop_assum mp_tac>>
     TOP_CASE_TAC>>rw[]>>
-    first_x_assum (irule_at Any)>>fs[constraint_TYPE_def]>>
+    first_x_assum (irule_at Any)>>
     metis_tac[EqualityType_NUM_BOOL])
 QED
 
@@ -207,7 +231,7 @@ QED
 val r = translate (lslack_def |> SIMP_RULE std_ss [MEMBER_INTRO, o_DEF]);
 val r = translate (check_contradiction_def |> SIMP_RULE std_ss[LET_DEF]);
 
-(* TODO:  can use Unsafe.update instead of Array.update *)
+(* TODO: can use Unsafe.update instead of Array.update *)
 val list_delete_arr = process_topdecs`
   fun list_delete_arr ls fml =
     case ls of
@@ -345,7 +369,7 @@ Proof
   xmatch
   >- (xcon>>xsimpl)>>
   xapp>>xsimpl>>
-  metis_tac[constraint_TYPE_def]
+  metis_tac[]
 QED
 
 (* TODO: copied *)
@@ -407,7 +431,7 @@ val check_lstep_arr = process_topdecs`
         check_lsteps_arr lno ss core fml' inds' mindel id'
 ` |> append_prog
 
-val NPBC_CHECK_LSTEP_TYPE_def = fetch "-" "NPBC_CHECK_LSTEP_TYPE_def"
+val NPBC_CHECK_LSTEP_TYPE_def = fetch "-" "NPBC_CHECK_LSTEP_TYPE_def";
 
 Theorem ARRAY_refl:
   (ARRAY fml fmllsv ==>> ARRAY fml fmllsv) ∧
@@ -521,7 +545,6 @@ Proof
       qexists_tac`lss`>>xsimpl>>
       simp[Abbr`lss`]>>
       match_mp_tac LIST_REL_update_resize>>simp[]>>
-      fs[constraint_TYPE_def]>>
       EVAL_TAC>>
       metis_tac[])
     >- ( (* Con *)
@@ -537,10 +560,8 @@ Proof
       `LIST_REL (OPTION_TYPE constraint_TYPE)
         (update_resize fmlls NONE (SOME (not p')) id)
         (update_resize fmllsv (Conv (SOME (TypeStamp "None" 2)) [])
-                (Conv (SOME (TypeStamp "Some" 2)) [v]) id)` by
-        (
-        match_mp_tac LIST_REL_update_resize>>fs[OPTION_TYPE_def]>>
-        fs[constraint_TYPE_def])>>
+                (Conv (SOME (TypeStamp "Some" 2)) [v]) id)` by (
+        match_mp_tac LIST_REL_update_resize>>fs[OPTION_TYPE_def])>>
       disch_then drule>>
       disch_then drule>>
       strip_tac>>
@@ -565,8 +586,7 @@ Proof
         qexists_tac`ls`>>xsimpl>>
         simp[Abbr`ls`]>>
         match_mp_tac LIST_REL_update_resize>>
-        simp[OPTION_TYPE_def]>>
-        fs[constraint_TYPE_def])>>
+        simp[OPTION_TYPE_def])>>
       xmatch>>
       rpt xlet_autop>>
       xif>>asm_exists_tac>>xsimpl>>
@@ -588,7 +608,6 @@ Proof
         rpt xlet_autop>>
         xraise>> xsimpl>>
         metis_tac[Fail_exn_def,ARRAY_refl]) >>
-      fs[constraint_TYPE_def]>>
       xlet_autop>>
       xif>>rpt xlet_autop
       >- (
@@ -742,12 +761,16 @@ val extract_clauses_arr = process_topdecs`
       else raise Fail (format_failure lno ("invalid #proofgoal id: " ^ Int.toString u))
 ` |> append_prog;
 
+Overload "subst_TYPE" = ``(VECTOR_TYPE (OPTION_TYPE (SUM_TYPE BOOL (PBC_LIT_TYPE NUM))))``
+
+Overload "pfs_TYPE" = ``LIST_TYPE (PAIR_TYPE (OPTION_TYPE (PAIR_TYPE (SUM_TYPE NUM NUM) NUM)) (LIST_TYPE NPBC_CHECK_LSTEP_TYPE))``
+
 Theorem extract_clauses_arr_spec:
   ∀pfs pfsv s sv fmlls fmlv fmllsv rsubs rsubsv acc accv lno lnov.
   NUM lno lnov ∧
-  (VECTOR_TYPE (OPTION_TYPE (SUM_TYPE BOOL (PBC_LIT_TYPE NUM)))) s sv ∧
+  subst_TYPE s sv ∧
   LIST_TYPE (LIST_TYPE constraint_TYPE) rsubs rsubsv ∧
-  LIST_TYPE (PAIR_TYPE (OPTION_TYPE (PAIR_TYPE (SUM_TYPE NUM NUM) NUM)) (LIST_TYPE NPBC_CHECK_LSTEP_TYPE)) pfs pfsv ∧
+  pfs_TYPE pfs pfsv ∧
   LIST_TYPE (PAIR_TYPE (OPTION_TYPE (PAIR_TYPE (LIST_TYPE constraint_TYPE) NUM)) (LIST_TYPE NPBC_CHECK_LSTEP_TYPE)) acc accv ∧
   LIST_REL (OPTION_TYPE constraint_TYPE) fmlls fmllsv
   ⇒
@@ -808,7 +831,6 @@ Proof
       simp[extract_clauses_list_def]>>
       metis_tac[Fail_exn_def])>>
     xmatch>>
-    fs[constraint_TYPE_def]>>
     rpt xlet_autop>>
     xapp>>
     xsimpl>>
@@ -819,7 +841,6 @@ Proof
     simp[extract_clauses_list_def]>>
     simp[LIST_TYPE_def,PAIR_TYPE_def,OPTION_TYPE_def,Abbr`acc'`])>>
   (* INR *)
-  fs[constraint_TYPE_def]>>
   rpt xlet_autop>>
   IF_CASES_TAC>>xif>>asm_exists_tac>>simp[]
   >- (
@@ -859,7 +880,7 @@ val subst_indexes_arr = process_topdecs`
 
 Theorem subst_indexes_arr_spec:
   ∀is isv s sv fmlls fmllsv fmlv.
-  (VECTOR_TYPE (OPTION_TYPE (SUM_TYPE BOOL (PBC_LIT_TYPE NUM)))) s sv ∧
+  subst_TYPE s sv ∧
   LIST_TYPE NUM is isv ∧
   LIST_REL (OPTION_TYPE constraint_TYPE) fmlls fmllsv
   ⇒
@@ -891,7 +912,6 @@ Proof
     xmatch>>xapp>>
     metis_tac[])>>
   xmatch>>
-  fs[constraint_TYPE_def]>>
   xlet_autop>>
   TOP_CASE_TAC>>fs[OPTION_TYPE_def]
   >- (
@@ -1123,7 +1143,7 @@ Proof
     xmatch>>
     xcon>>xsimpl) >>
   xmatch>>
-  fs[constraint_TYPE_def]>>
+  fs[]>>
   rpt xlet_autop>>
   xlet_auto>- (
     xsimpl>>
@@ -1161,7 +1181,7 @@ Theorem in_hashset_arr_spec:
 Proof
   rw[]>>simp[in_hashset_def]>>
   xcf "in_hashset_arr" (get_ml_prog_state ())>>
-  fs[constraint_TYPE_def]>>
+  fs[]>>
   xlet_autop>>
   xlet_auto
   >- (xsimpl>>simp[hash_constraint_splim])>>
@@ -1344,7 +1364,7 @@ Theorem red_cond_check_spec:
 Proof
   rw[]>>
   xcf "red_cond_check" (get_ml_prog_state ())>>
-  fs[constraint_TYPE_def]>>
+  fs[]>>
   xlet_autop>>
   simp[red_cond_check_eq]>>
   TOP_CASE_TAC>>fs[OPTION_TYPE_def]
@@ -1355,7 +1375,7 @@ Proof
   xmatch>>
   xapp>>
   xsimpl>>
-  fs[constraint_TYPE_def]>>
+  fs[]>>
   first_x_assum (irule_at Any)>>
   first_x_assum (irule_at Any)>>
   first_x_assum (irule_at Any)>>
@@ -1400,13 +1420,9 @@ val format_failure_2_def = Define`
 
 val r = translate format_failure_2_def;
 
-val check_sstep_arr = process_topdecs`
-  fun check_sstep_arr lno step ord obj core fml inds id =
-  case step of
-    Lstep lstep =>
-    check_lstep_arr lno lstep core fml inds 0 id
-  | Red c s pfs idopt =>
-    ( case reindex_arr fml inds of (rinds,fmlls) =>
+val check_red_arr = process_topdecs`
+  fun check_red_arr lno ord obj core fml inds id c s pfs idopt =
+  (case reindex_arr fml inds of (rinds,fmlls) =>
       let val rsubs = do_rso ord s c obj
          val cpfs = extract_clauses_arr lno s fml rsubs pfs []
          val fml_not_c = Array.updateResize fml None id (Some (not_1 c)) in
@@ -1418,43 +1434,170 @@ val check_sstep_arr = process_topdecs`
                val goals = subst_indexes_arr s fml' rinds in
                if red_cond_check fmlls pfs rsubs goals
                then
-                 (Array.updateResize fml' None id' (Some c), ((id'+1), sorted_insert id' rinds))
+                 (fml', (id', rinds))
                else raise Fail (format_failure_2 lno ("Redundancy subproofs did not cover all subgoals.") (print_subproofs_err rsubs goals))
            end
         | Some cid =>
           if check_contradiction_fml_arr fml' cid then
             let val u = rollback_arr fml' id id' in
-              (Array.updateResize fml' None id' (Some c), ((id'+1), sorted_insert id' rinds))
+              (fml', (id', rinds))
             end
           else raise Fail (format_failure lno ("did not derive contradiction from index:" ^ Int.toString cid)))
-    end)
+    end)` |> append_prog;
+
+(* Overloads all the _TYPEs that we will reuse *)
+Overload "spo_TYPE" = ``PAIR_TYPE
+      (LIST_TYPE constraint_TYPE)
+      (PAIR_TYPE (LIST_TYPE NUM) (LIST_TYPE NUM))``
+
+Overload "ord_TYPE" = ``
+  OPTION_TYPE (PAIR_TYPE spo_TYPE (LIST_TYPE NUM))``
+
+Overload "obj_TYPE" = ``
+  OPTION_TYPE (PAIR_TYPE (LIST_TYPE (PAIR_TYPE INT NUM)) INT)``
+
+Theorem check_red_arr_spec:
+  NUM lno lnov ∧
+  ord_TYPE ord ordv ∧
+  obj_TYPE obj objv ∧
+  SPTREE_SPT_TYPE UNIT_TYPE core corev ∧
+  LIST_REL (OPTION_TYPE constraint_TYPE) fmlls fmllsv ∧
+  (LIST_TYPE NUM) inds indsv ∧
+  NUM id idv ∧
+  constraint_TYPE c cv ∧
+  subst_TYPE s sv ∧
+  pfs_TYPE pfs pfsv ∧
+  OPTION_TYPE NUM idopt idoptv
+  ⇒
+  app (p : 'ffi ffi_proj)
+    ^(fetch_v "check_red_arr" (get_ml_prog_state()))
+    [lnov; ordv; objv; corev; fmlv; indsv; idv;
+      cv; sv; pfsv; idoptv]
+    (ARRAY fmlv fmllsv)
+    (POSTve
+      (λv.
+        SEP_EXISTS fmlv' fmllsv'.
+        ARRAY fmlv' fmllsv' *
+        &(
+          case check_red_list ord obj core fmlls inds id
+              c s pfs idopt of NONE => F
+          | SOME res =>
+            PAIR_TYPE (λl v.
+              LIST_REL (OPTION_TYPE constraint_TYPE) l fmllsv' ∧
+              v = fmlv') (PAIR_TYPE NUM (LIST_TYPE NUM)) res v
+          ))
+      (λe.
+        SEP_EXISTS fmlv' fmllsv'.
+        ARRAY fmlv' fmllsv' *
+        & (Fail_exn e ∧
+          check_red_list ord obj core fmlls inds id
+              c s pfs idopt = NONE)))
+Proof
+  rw[]>>
+  xcf "check_red_arr" (get_ml_prog_state ())>>
+  rw[check_red_list_def]>>
+  xlet_autop>>
+  pairarg_tac>>gs[]>>
+  fs[PAIR_TYPE_def]>>
+  xmatch>>
+  rpt xlet_autop>>
+  qmatch_asmsub_abbrev_tac`VECTOR_TYPE _ s _`>>
+  qmatch_goalsub_abbrev_tac`ARRAY aa vv`>>
+  xlet`(POSTve
+    (λv.
+      ARRAY aa vv *
+      &(case extract_clauses_list s fmlls (do_rso ord s c obj) pfs [] of
+          NONE => F
+        | SOME res => LIST_TYPE (PAIR_TYPE (OPTION_TYPE (PAIR_TYPE (LIST_TYPE constraint_TYPE) NUM)) (LIST_TYPE NPBC_CHECK_LSTEP_TYPE)) res v))
+  (λe.
+    ARRAY aa vv *
+    & (Fail_exn e ∧ extract_clauses_list s fmlls (do_rso ord s c obj) pfs [] = NONE)))`
+  >- (
+    xapp>>xsimpl>>
+    fs[LIST_TYPE_def]>>
+    metis_tac[])
+  >- (
+    xsimpl>>
+    fs[do_rso_def]>>
+    metis_tac[ARRAY_refl])>>
+  fs[]>>
+  pop_assum mp_tac>>TOP_CASE_TAC>>gvs[]>>
+  strip_tac>>
+  fs[do_rso_def]>>
+  rpt xlet_autop>>
+  xlet_auto>>
+  rpt xlet_autop>>
+  rename1`_ (not n) vvv`>>
+  `LIST_REL (OPTION_TYPE constraint_TYPE)
+    (update_resize fmlls NONE (SOME (not n)) id)
+    (update_resize fmllsv (Conv (SOME (TypeStamp "None" 2)) [])
+            (Conv (SOME (TypeStamp "Some" 2)) [vvv]) id)` by
+    (match_mp_tac LIST_REL_update_resize>>fs[OPTION_TYPE_def])>>
+  xlet_autop
+  >- (
+    xsimpl>>rw[]>>
+    fs[do_rso_def]>>
+    metis_tac[ARRAY_refl])>>
+  pop_assum mp_tac>>
+  TOP_CASE_TAC>>fs[]>>
+  Cases_on`x'`>>simp[PAIR_TYPE_def]>>
+  strip_tac>>
+  xmatch>>
+  Cases_on`idopt`>>fs[OPTION_TYPE_def,do_red_check_def]>>xmatch
+  >- (
+    rpt xlet_autop>>
+    fs[do_red_check_def]>>
+    reverse xif
+    >- (
+      rpt xlet_autop>>
+      fs[red_cond_check_def]>>
+      xraise>>
+      xsimpl>>
+      rw[]>>fs[]>>
+      metis_tac[ARRAY_refl,NOT_EVERY,Fail_exn_def]) >>
+    fs[red_cond_check_def]>>
+    pairarg_tac>>fs[]>>
+    xlet_autop>>
+    xcon>>xsimpl>>
+    simp[PAIR_TYPE_def]>>
+    xsimpl)>>
+  rpt xlet_autop>>
+  reverse xif
+  >- (
+    rpt xlet_autop>>
+    xraise>>
+    xsimpl>>
+    rw[]>>fs[]>>
+    metis_tac[ARRAY_refl,NOT_EVERY,Fail_exn_def]) >>
+  rpt xlet_autop>>
+  xcon>>xsimpl>>
+  simp[PAIR_TYPE_def]>>
+  xsimpl
+QED
+
+val check_sstep_arr = process_topdecs`
+  fun check_sstep_arr lno step ord obj core fml inds id =
+  case step of
+    Lstep lstep =>
+    check_lstep_arr lno lstep core fml inds 0 id
+  | Red c s pfs idopt =>
+    (case check_red_arr lno ord obj core
+        fml inds id c s pfs idopt of (fml',(id',rinds)) =>
+       (Array.updateResize fml' None id' (Some c),
+        ((id'+1), sorted_insert id' rinds)))
   ` |> append_prog
 
 val NPBC_CHECK_SSTEP_TYPE_def = theorem "NPBC_CHECK_SSTEP_TYPE_def";
 
-Definition spo_TYPE_def:
-  spo_TYPE =
-    (PAIR_TYPE
-      (LIST_TYPE constraint_TYPE)
-      (PAIR_TYPE (LIST_TYPE NUM) (LIST_TYPE NUM)))
-End
-
-Definition ord_TYPE_def:
-  ord_TYPE =
-  OPTION_TYPE
-     (PAIR_TYPE spo_TYPE (LIST_TYPE NUM))
-End
-
 Theorem check_sstep_arr_spec:
-  ∀step fmlls inds id stepv lno lnov idv indsv fmlv fmllsv obj objv core corev ord ordv.
-  NPBC_CHECK_SSTEP_TYPE step stepv ∧
   NUM lno lnov ∧
-  SPTREE_SPT_TYPE UNIT_TYPE core corev ∧
-  OPTION_TYPE (LIST_TYPE (PAIR_TYPE INT NUM)) obj objv ∧
+  NPBC_CHECK_SSTEP_TYPE step stepv ∧
   ord_TYPE ord ordv ∧
-  NUM id idv ∧
+  obj_TYPE obj objv ∧
+  SPTREE_SPT_TYPE UNIT_TYPE core corev ∧
   LIST_REL (OPTION_TYPE constraint_TYPE) fmlls fmllsv ∧
-  (LIST_TYPE NUM) inds indsv
+  (LIST_TYPE NUM) inds indsv ∧
+  NUM id idv
   ⇒
   app (p : 'ffi ffi_proj)
     ^(fetch_v "check_sstep_arr" (get_ml_prog_state()))
@@ -1488,99 +1631,18 @@ Proof
     metis_tac[])
   >- ((*Red*)
     xmatch>>
-    pairarg_tac>>gs[]>>
-    xlet_autop>>
-    fs[PAIR_TYPE_def]>>
-    xmatch>>
-    rpt xlet_autop>>
-    fs[spo_TYPE_def,ord_TYPE_def,constraint_TYPE_def]>>
-    rpt xlet_autop>>
-    qmatch_asmsub_abbrev_tac`VECTOR_TYPE _ s _`>>
-    qmatch_goalsub_abbrev_tac`ARRAY aa vv`>>
-    xlet`(POSTve
-      (λv.
-        ARRAY aa vv *
-        &(case extract_clauses_list s fmlls (do_rso ord s p' obj) l [] of
-            NONE => F
-          | SOME res => LIST_TYPE (PAIR_TYPE (OPTION_TYPE (PAIR_TYPE (LIST_TYPE constraint_TYPE) NUM)) (LIST_TYPE NPBC_CHECK_LSTEP_TYPE)) res v))
-    (λe.
-      ARRAY aa vv *
-      & (Fail_exn e ∧ extract_clauses_list s fmlls (do_rso ord s p' obj) l [] = NONE)))`
-    >- (
-      xapp>>xsimpl>>
-      fs[constraint_TYPE_def,LIST_TYPE_def]>>
-      metis_tac[])
-    >- (
-      xsimpl>>
-      fs[do_rso_def]>>
-      metis_tac[ARRAY_refl])>>
-    fs[]>>
-    pop_assum mp_tac>>TOP_CASE_TAC>>gvs[]>>
-    strip_tac>>
-    fs[do_rso_def]>>
-    rpt xlet_autop>>
-    xlet_auto>>
-    rpt xlet_autop>>
-    rename1`_ (not n) vvv`>>
-    `LIST_REL (OPTION_TYPE constraint_TYPE)
-      (update_resize fmlls NONE (SOME (not n)) id)
-      (update_resize fmllsv (Conv (SOME (TypeStamp "None" 2)) [])
-              (Conv (SOME (TypeStamp "Some" 2)) [vvv]) id)` by
-      (match_mp_tac LIST_REL_update_resize>>fs[OPTION_TYPE_def,constraint_TYPE_def])>>
     xlet_autop
     >- (
-      xsimpl>>rw[]>>
-      fs[do_rso_def]>>
-      metis_tac[ARRAY_refl])>>
-    pop_assum mp_tac>>
-    TOP_CASE_TAC>>fs[]>>
-    Cases_on`x'`>>simp[PAIR_TYPE_def]>>
-    strip_tac>>
-    xmatch>>
-    rename1`OPTION_TYPE NUM idopt _`>>
-    Cases_on`idopt`>>fs[OPTION_TYPE_def,do_red_check_def]>>xmatch
-    >- (
-      rpt xlet_autop>>
-      fs[GSYM constraint_TYPE_def]>>
-      xlet_autop>>
-      fs[do_red_check_def]>>
-      reverse xif
-      >- (
-        rpt xlet_autop>>
-        fs[red_cond_check_def]>>
-        pairarg_tac>>fs[]>>
-        xraise>>
-        xsimpl>>
-        rw[]>>fs[]>>
-        metis_tac[ARRAY_refl,NOT_EVERY,Fail_exn_def]) >>
-      fs[red_cond_check_def]>>
-      pairarg_tac>>fs[]>>
-      rpt xlet_autop>>
-      xlet_auto>>
-      xcon>>xsimpl>>
-      simp[PAIR_TYPE_def]>>
-      qmatch_goalsub_abbrev_tac`ARRAY _ vvvv`>>
-      qexists_tac`vvvv`>>xsimpl>>
-      simp[Abbr`vvvv`]>>
-      match_mp_tac LIST_REL_update_resize>>
-      fs[OPTION_TYPE_def,constraint_TYPE_def])>>
-    rpt xlet_autop>>
-    reverse xif
-    >- (
-      rpt xlet_autop>>
-      xraise>>
       xsimpl>>
-      rw[]>>fs[]>>
-      metis_tac[ARRAY_refl,NOT_EVERY,Fail_exn_def]) >>
+      rw[]>>
+      metis_tac[ARRAY_refl])>>
+    every_case_tac>>fs[PAIR_TYPE_def]>>
+    xmatch>>
     rpt xlet_autop>>
     xlet_auto>>
     xcon>>xsimpl>>
-    simp[PAIR_TYPE_def]>>
-    qmatch_goalsub_abbrev_tac`ARRAY _ vvvv`>>
-    qexists_tac`vvvv`>>xsimpl>>
-    simp[Abbr`vvvv`]>>
     match_mp_tac LIST_REL_update_resize>>
-    fs[OPTION_TYPE_def,constraint_TYPE_def])
+    simp[OPTION_TYPE_def])
 QED
 
 val read_coref_arr = process_topdecs`
@@ -1588,7 +1650,7 @@ val read_coref_arr = process_topdecs`
   case ls of [] => []
   | i::is =>
     case Array.lookup fml None i of
-      None => (i,([],0))::read_coref_arr is fml
+      None => read_coref_arr is fml
     | Some res => (i,res) :: read_coref_arr is fml` |> append_prog
 
 Theorem read_coref_arr_spec:
@@ -1611,7 +1673,7 @@ Proof
   fs[LIST_TYPE_def]>>xmatch
   >-
     (xcon>>xsimpl)>>
-  xlet_autop>>
+  rpt xlet_autop>>
   xlet_auto>>
   `OPTION_TYPE constraint_TYPE (any_el h fmlls NONE) v'` by (
    rw[any_el_ALT]>>
@@ -1620,18 +1682,14 @@ Proof
   TOP_CASE_TAC>>gs[OPTION_TYPE_def]>>
   xmatch
   >- (
-    first_x_assum drule>>
-    rw[]>>
-    rpt xlet_autop>>
-    xcon>>
-    xsimpl>>
-    fs[LIST_TYPE_def,PAIR_TYPE_def,constraint_TYPE_def])>>
+    xapp>>
+    fs[LIST_TYPE_def,PAIR_TYPE_def])>>
   first_x_assum drule>>
   rw[]>>
   rpt xlet_autop>>
   xcon>>
   xsimpl>>
-  fs[LIST_TYPE_def,PAIR_TYPE_def,constraint_TYPE_def]
+  fs[LIST_TYPE_def,PAIR_TYPE_def]
 QED
 
 val res = translate lrnext_def;
@@ -1804,9 +1862,16 @@ val res = translate npbc_checkTheory.opt_lt_def;
 val res = translate npbcTheory.satisfies_npbc_def;
 val res = translate npbc_checkTheory.check_obj_def;
 
+val res = translate npbc_checkTheory.nn_int_def;
+val nn_int_side = Q.prove(
+  `∀x. nn_int_side x`,
+  EVAL_TAC>>
+  intLib.ARITH_TAC
+  ) |> update_precondition
+
 val res = translate npbc_checkTheory.model_improving_def;
 
-(* Pure part of checked_del chk=T *)
+(* TODO Pure part of checked_del chk=T
 Definition checked_del_pure_chk_def:
   checked_del_pure_chk cf pfs ord obj core id inds ls bound orders =
   case check_del pfs ord obj core cf id of
@@ -1820,6 +1885,7 @@ Definition checked_del_pure_chk_def:
   else
     NONE
 End
+ *)
 
 Definition do_dso_def:
   do_dso spo s c obj =
@@ -1846,15 +1912,128 @@ End
 val res = translate do_core_del_def;
 val res = translate core_from_inds_def;
 
-val check_cstep_arr = process_topdecs`
-  fun check_cstep_arr lno cstep chk ord obj bound
-    core fml inds id orders =
-  case cstep of
-    Dom c s pfs idopt =>
-    (case ord of None =>
-      raise Fail (format_failure lno "no order loaded for dominance")
-    | Some spo =>
-    case reindex_arr fml inds of (rinds,fmlls) =>
+Definition check_change_obj_pure_def:
+  check_change_obj_pure core chk obj ord fc' n1 fc c1 c2 =
+  ((chk ∨ IS_SOME ord ⇒ sptree$lookup n1 core = SOME ()) ∧
+  imp c1 (model_bounding fc fc') ∧
+  imp c2 (model_bounding fc' fc))
+End
+
+val res = translate npbc_checkTheory.model_bounding_def;
+val res = translate check_change_obj_pure_def;
+
+val check_change_obj_arr = process_topdecs`
+  fun check_change_obj_arr lno fml core chk obj ord fc' n1 n2 =
+  case obj of None =>
+    raise Fail (format_failure lno ("no objective loaded"))
+  | Some fc =>
+    (case Array.lookup fml None n1 of
+      None => raise Fail (format_failure lno
+          ("invalid constraint ID in objective update"))
+    | Some c1 =>
+      (case Array.lookup fml None n2 of
+      None => raise Fail (format_failure lno
+          ("invalid constraint ID in objective update"))
+    | Some c2 =>
+      if check_change_obj_pure core chk obj ord fc' n1 fc c1 c2
+      then ()
+      else
+      raise Fail (format_failure lno ("objective update check failed"))))` |> append_prog;
+
+Theorem check_change_obj_arr_spec:
+  NUM lno lnov ∧
+  LIST_REL (OPTION_TYPE constraint_TYPE) fmlls fmllsv ∧
+  SPTREE_SPT_TYPE UNIT_TYPE core corev ∧
+  BOOL chk chkv ∧
+  obj_TYPE obj objv ∧
+  ord_TYPE ord ordv ∧
+  PAIR_TYPE (LIST_TYPE (PAIR_TYPE INT NUM)) INT fc fcv ∧
+  NUM n1 n1vv ∧
+  NUM n2 n2vv
+  ⇒
+  app (p : 'ffi ffi_proj)
+    ^(fetch_v "check_change_obj_arr" (get_ml_prog_state()))
+    [lnov; fmlv; corev; chkv; objv; ordv; fcv; n1vv; n2vv]
+    (ARRAY fmlv fmllsv)
+    (POSTve
+      (λv.
+      ARRAY fmlv fmllsv *
+        &(check_change_obj_list fmlls core
+          chk obj ord fc n1 n2))
+      (λe.
+      ARRAY fmlv fmllsv *
+        &(Fail_exn e ∧
+          ¬check_change_obj_list fmlls core
+          chk obj ord fc n1 n2 )))
+Proof
+  rw[]>>
+  xcf "check_change_obj_arr" (get_ml_prog_state ())>>
+  simp[check_change_obj_list_def]>>
+  Cases_on`obj`>>fs[OPTION_TYPE_def]>>xmatch
+  >- (
+    rpt xlet_autop>>
+    xraise>>xsimpl>>
+    metis_tac[Fail_exn_def])>>
+  rpt xlet_autop>>
+  xlet_auto>>
+  rename1`cv1 = any_el n1 _ _`>>
+  `OPTION_TYPE constraint_TYPE (any_el n1 fmlls NONE) cv1` by (
+    rw[any_el_ALT]>>
+    fs[LIST_REL_EL_EQN,OPTION_TYPE_def])>>
+  qpat_x_assum`cv1 = _` (assume_tac o SYM)>>
+  TOP_CASE_TAC>>
+  fs[OPTION_TYPE_def]>>xmatch
+  >- (
+    rpt xlet_autop>>
+    xraise>>xsimpl>>
+    metis_tac[Fail_exn_def])>>
+  rpt xlet_autop>>
+  xlet_auto>>
+  rename1`cv2 = any_el n2 _ _`>>
+  `OPTION_TYPE constraint_TYPE (any_el n2 fmlls NONE) cv2` by (
+    rw[any_el_ALT]>>
+    fs[LIST_REL_EL_EQN,OPTION_TYPE_def])>>
+  qpat_x_assum`cv2 = _` (assume_tac o SYM)>>
+  TOP_CASE_TAC>>
+  fs[OPTION_TYPE_def]>>xmatch
+  >- (
+    rpt xlet_autop>>
+    xraise>>xsimpl>>
+    metis_tac[Fail_exn_def])>>
+  xlet_autop>>
+  xif
+  >- (
+    fs[check_change_obj_pure_def] >>
+    xcon>>xsimpl>>
+    metis_tac[])>>
+  rpt xlet_autop>>
+  xraise>>xsimpl>>
+  fs[check_change_obj_pure_def]>>
+  metis_tac[Fail_exn_def]
+QED
+
+Definition check_dom_list_def:
+  check_dom_list spo obj core fml inds id c s pfs idopt =
+  let (rinds,fmlls) = reindex fml inds in
+  let fml_not_c = update_resize fml NONE (SOME (not c)) id in
+  let w = subst_fun s in
+  let cf = coref_list core fml in
+  let dsubs = dom_subgoals spo w c obj in
+  case extract_clauses_list s fml dsubs pfs [] of
+    NONE => NONE
+  | SOME cpfs =>
+    (case check_subproofs_list cpfs core fml_not_c (sorted_insert id rinds) id (id+1) of
+      NONE => NONE
+    | SOME (fml',id') =>
+      let rfml = rollback fml' id id' in
+      if do_dom_check idopt fml' rfml w cf fmlls pfs dsubs then
+        SOME (rfml,id',rinds)
+      else NONE)
+End
+
+val check_dom_arr = process_topdecs`
+  fun check_dom_arr lno spo obj core fml inds id c s pfs idopt =
+  (case reindex_arr fml inds of (rinds,fmlls) =>
     let
         val cf = coref_arr core fml
         val dsubs = do_dso spo s c obj
@@ -1868,20 +2047,257 @@ val check_cstep_arr = process_topdecs`
                  val goals = core_subgoals s cf in
                  if red_cond_check fmlls pfs dsubs goals
                  then
-                   (Array.updateResize fml' None id' (Some c),
-                   (sorted_insert id' rinds,
-                   (id'+1, (core, (bound, (ord,orders))))))
+                   (fml',(id',rinds))
                  else raise Fail (format_failure_2 lno ("Dominance subproofs did not cover all subgoals") (print_subproofs_err dsubs goals))
              end
            | Some cid =>
              if check_contradiction_fml_arr fml' cid then
                let val u = rollback_arr fml' id id' in
-                 (Array.updateResize fml' None id' (Some c),
-                   (sorted_insert id' rinds,
-                   (id'+1, (core, (bound, (ord,orders))))))
+                 (fml', (id', rinds))
                end
              else raise Fail (format_failure lno ("did not derive contradiction from index:" ^ Int.toString cid)))
-    end)
+    end)` |> append_prog;
+
+Theorem check_dom_arr_spec:
+  NUM lno lnov ∧
+  PAIR_TYPE spo_TYPE (LIST_TYPE NUM) spo spov ∧
+  obj_TYPE obj objv ∧
+  SPTREE_SPT_TYPE UNIT_TYPE core corev ∧
+  LIST_REL (OPTION_TYPE constraint_TYPE) fmlls fmllsv ∧
+  (LIST_TYPE NUM) inds indsv ∧
+  NUM id idv ∧
+  constraint_TYPE c cv ∧
+  subst_TYPE s sv ∧
+  pfs_TYPE pfs pfsv ∧
+  OPTION_TYPE NUM idopt idoptv
+  ⇒
+  app (p : 'ffi ffi_proj)
+    ^(fetch_v "check_dom_arr" (get_ml_prog_state()))
+    [lnov; spov; objv; corev; fmlv; indsv; idv;
+      cv; sv; pfsv; idoptv]
+    (ARRAY fmlv fmllsv)
+    (POSTve
+      (λv.
+        SEP_EXISTS fmlv' fmllsv'.
+        ARRAY fmlv' fmllsv' *
+        &(
+          case check_dom_list spo obj core fmlls inds id
+              c s pfs idopt of NONE => F
+          | SOME res =>
+            PAIR_TYPE (λl v.
+              LIST_REL (OPTION_TYPE constraint_TYPE) l fmllsv' ∧
+              v = fmlv') (PAIR_TYPE NUM (LIST_TYPE NUM)) res v
+          ))
+      (λe.
+        SEP_EXISTS fmlv' fmllsv'.
+        ARRAY fmlv' fmllsv' *
+        & (Fail_exn e ∧
+          check_dom_list spo obj core fmlls inds id
+              c s pfs idopt = NONE)))
+Proof
+  rw[]>>
+  xcf "check_dom_arr" (get_ml_prog_state ())>>
+  rw[check_dom_list_def]>>
+  pairarg_tac>>xlet_autop>>
+  fs[PAIR_TYPE_def]>>
+  xmatch>>
+  rpt xlet_autop>>
+  xlet`(POSTve
+    (λv.
+      ARRAY fmlv fmllsv *
+      &(case extract_clauses_list s fmlls (do_dso spo s c obj) pfs [] of
+          NONE => F
+        | SOME res => LIST_TYPE (PAIR_TYPE (OPTION_TYPE (PAIR_TYPE (LIST_TYPE constraint_TYPE) NUM)) (LIST_TYPE NPBC_CHECK_LSTEP_TYPE)) res v))
+  (λe.
+    ARRAY fmlv fmllsv *
+    & (Fail_exn e ∧ extract_clauses_list s fmlls (do_dso spo s c obj) pfs [] = NONE)))`
+  >- (
+    xapp>>xsimpl>>
+    simp[LIST_TYPE_def]>>
+    metis_tac[])
+  >- (
+    xsimpl>>
+    simp[do_dso_def]>>
+    metis_tac[ARRAY_refl])>>
+  pop_assum mp_tac>>TOP_CASE_TAC>>simp[]>>
+  fs[do_dso_def]>>
+  strip_tac>>
+  rpt xlet_autop>>
+  xlet_auto>>
+  rpt xlet_autop>>
+  rename1`_ (not n) vvv`>>
+  `LIST_REL (OPTION_TYPE constraint_TYPE)
+    (update_resize fmlls NONE (SOME (not n)) id)
+    (update_resize fmllsv (Conv (SOME (TypeStamp "None" 2)) [])
+            (Conv (SOME (TypeStamp "Some" 2)) [vvv]) id)` by (
+    match_mp_tac LIST_REL_update_resize>>
+    fs[OPTION_TYPE_def])>>
+  xlet_autop
+  >- (
+    xsimpl>>rw[]>>
+    metis_tac[ARRAY_refl])>>
+  pop_assum mp_tac>>
+  TOP_CASE_TAC>>fs[]>>
+  Cases_on`x'`>>simp[PAIR_TYPE_def]>>
+  strip_tac>>
+  xmatch>>
+  Cases_on`idopt`>>
+  fs[OPTION_TYPE_def,do_dom_check_def]>>
+  xmatch
+  >- (
+    rpt xlet_autop>>
+    reverse xif>>gs[]
+    >- (
+      rpt xlet_autop>>
+      fs[red_cond_check_def]>>pairarg_tac>>fs[core_subgoals_def]>>
+      xraise>>xsimpl>>
+      fs[red_cond_check_def]>>rw[]>>
+      metis_tac[ARRAY_refl,Fail_exn_def,NOT_EVERY])>>
+    xlet_autop>>
+    xcon>>xsimpl>>
+    pairarg_tac>>fs[red_cond_check_def,core_subgoals_def]>>
+    fs[PAIR_TYPE_def,OPTION_TYPE_def]>>
+    xsimpl)>>
+  rpt xlet_autop>>
+  reverse xif
+  >- (
+    rpt xlet_autop>>
+    xraise>>
+    xsimpl>>
+    rw[]>>fs[]>>
+    metis_tac[ARRAY_refl,NOT_EVERY,Fail_exn_def])>>
+  rpt xlet_autop>>
+  xcon>>xsimpl>>
+  simp[PAIR_TYPE_def]>>
+  xsimpl
+QED
+
+val load_coref_arr = process_topdecs`
+  fun load_coref_arr ls fml newfml =
+  case ls of [] => ()
+  | i::is =>
+    if Array.length fml <= i
+    then load_coref_arr is fml newfml
+    else
+      (Array.update newfml i
+        (Array.sub fml i);
+        load_coref_arr is fml newfml)` |> append_prog;
+
+Theorem LUPDATE_outside:
+  ∀ls n.
+  LENGTH ls ≤ n ⇒
+  LUPDATE v n ls = ls
+Proof
+  Induct>>rw[LUPDATE_DEF]
+QED
+
+Theorem load_coref_arr_spec:
+  ∀ls lsv nfmlls nfmllsv.
+  LIST_TYPE NUM ls lsv ∧
+  LIST_REL (OPTION_TYPE constraint_TYPE) fmlls fmllsv ∧
+  LIST_REL (OPTION_TYPE constraint_TYPE) nfmlls nfmllsv ∧
+  LENGTH fmlls = LENGTH nfmlls
+  ⇒
+  app (p : 'ffi ffi_proj)
+    ^(fetch_v "load_coref_arr" (get_ml_prog_state()))
+    [lsv; fmlv; nfmlv]
+    (ARRAY fmlv fmllsv * ARRAY nfmlv nfmllsv)
+    (POSTv v.
+      SEP_EXISTS nfmllsv'.
+      ARRAY fmlv fmllsv *
+      ARRAY nfmlv nfmllsv' *
+      &(
+        LIST_REL (OPTION_TYPE constraint_TYPE)
+          (load_coref_list ls fmlls nfmlls)
+          nfmllsv'))
+Proof
+  Induct>>rw[load_coref_list_def]>>
+  xcf "load_coref_arr" (get_ml_prog_state ())>>
+  fs[LIST_TYPE_def]>>xmatch
+  >-
+    (xcon>>xsimpl)>>
+  rpt xlet_autop>>
+  xif
+  >- (
+    xapp>>xsimpl>>
+    DEP_REWRITE_TAC[LUPDATE_outside]>>
+    fs[LIST_REL_EL_EQN])>>
+  rpt xlet_autop>>
+  xlet_auto
+  >- (
+    xsimpl>>
+    fs[LIST_REL_EL_EQN])>>
+  xapp>>xsimpl>>
+  qexists_tac`LUPDATE (EL h fmlls) h nfmlls`>>simp[]>>
+  match_mp_tac EVERY2_LUPDATE_same>>
+  fs[LIST_REL_EL_EQN,any_el_ALT]
+QED
+
+val arr_from_core_arr = process_topdecs`
+  fun arr_from_core_arr core fml =
+  let val ids = mapfsttoalist core
+  val nfml = Array.array (Array.length fml) None
+  val u = load_coref_arr ids fml nfml in
+  (nfml, ids)
+  end` |> append_prog
+
+Theorem arr_from_core_arr_spec:
+  SPTREE_SPT_TYPE UNIT_TYPE core corev ∧
+  LIST_REL (OPTION_TYPE constraint_TYPE) fmlls fmllsv
+  ⇒
+  app (p : 'ffi ffi_proj)
+    ^(fetch_v "arr_from_core_arr" (get_ml_prog_state()))
+    [corev; fmlv]
+    (ARRAY fmlv fmllsv)
+    (POSTv v.
+      SEP_EXISTS nfmlv nfmllsv.
+      ARRAY fmlv fmllsv *
+      ARRAY nfmlv nfmllsv *
+      &(
+        PAIR_TYPE (λl v.
+              LIST_REL (OPTION_TYPE constraint_TYPE) l nfmllsv ∧
+              v = nfmlv) (LIST_TYPE NUM)
+          (arr_from_core_list core fmlls) v))
+Proof
+  xcf "arr_from_core_arr" (get_ml_prog_state ())>>
+  rpt xlet_autop>>
+  simp[arr_from_core_list_def]>>
+  xlet`POSTv v. SEP_EXISTS nfmllsv'.
+    ARRAY fmlv fmllsv * ARRAY av nfmllsv' *
+    &LIST_REL (OPTION_TYPE constraint_TYPE)
+      (load_coref_list (mapfsttoalist core)
+        fmlls (REPLICATE (LENGTH fmlls) NONE)) nfmllsv'`
+  >- (
+    xapp>>xsimpl>>
+    first_x_assum (irule_at Any)>>simp[]>>
+    first_assum (irule_at Any)>>simp[]>>
+    qexists_tac`REPLICATE (LENGTH fmlls) NONE`>>simp[]>>
+    `LENGTH fmlls  = LENGTH fmllsv` by
+      fs[LIST_REL_EL_EQN]>>
+    pop_assum SUBST_ALL_TAC>>
+    simp[LIST_REL_REPLICATE_same,OPTION_TYPE_def])>>
+  xcon>>xsimpl>>
+  simp[PAIR_TYPE_def]>>
+  fs[mapfsttoalist_def]>>
+  first_x_assum (irule_at Any)>>
+  xsimpl
+QED
+
+val check_cstep_arr = process_topdecs`
+  fun check_cstep_arr lno cstep core chk obj bound
+    ord orders fml inds id =
+  case cstep of
+    Dom c s pfs idopt => (
+    case ord of None =>
+      raise Fail (format_failure lno
+        "no order loaded for dominance")
+    | Some spo =>
+      case check_dom_arr lno spo obj
+        core fml inds id c s pfs idopt of (fml',(id',rinds)) =>
+      (Array.updateResize fml' None id' (Some c),
+       (sorted_insert id' rinds,
+       (id'+1,
+       (core,(chk,(obj,(bound,(ord,orders)))))))))
   | Loadorder nn xs =>
     let val inds' = fst (reindex_arr fml inds) in
     case Alist.lookup orders nn of
@@ -1889,18 +2305,22 @@ val check_cstep_arr = process_topdecs`
         raise Fail (format_failure lno ("no such order: " ^ nn))
     | Some ord' =>
       if List.length xs = List.length (fst (snd ord')) then
-        (fml,(inds',(id,(core_from_inds inds',(bound,(Some (ord',xs),orders))))))
+        (fml,(inds',(id,(core_from_inds inds',
+          (chk,(obj,(bound,(Some (ord',xs),orders))))))))
       else
-        raise Fail (format_failure lno ("invalid order instantiation"))
+        raise Fail
+          (format_failure lno ("invalid order instantiation"))
     end
   | Unloadorder =>
     (case ord of None =>
      raise Fail (format_failure lno ("no order loaded"))
     | Some spo =>
-      (fml,(inds,(id,(core,(bound,(None, orders)))))))
+      (fml,(inds,(id,(core,
+        (chk,(obj,(bound,(None, orders)))))))))
   | Storeorder nn spo ws pfs => (
     if check_storeorder spo ws pfs then
-      (fml,(inds,(id,(core,(bound,(ord,((nn,spo)::orders)))))))
+      (fml,(inds,(id,(core,
+        (chk,(obj,(bound,(ord,((nn,spo)::orders)))))))))
     else
      raise Fail (format_failure lno ("invalid order definition")))
   | Transfer ls => (
@@ -1908,36 +2328,46 @@ val check_cstep_arr = process_topdecs`
     then
       (fml, (inds, (id,
        (do_transfer core ls,
-       (bound, (ord, orders))))))
+       (chk,(obj,(bound, (ord, orders))))))))
     else
      raise Fail (format_failure lno ("core transfer invalid ids")))
-  | Checkeddelete ls pfs => (
-    if all_core_every core ls then
-    (
-      if chk then
-        raise Fail (format_failure lno ("core del with explicit subproofs not yet supported"))
-      else
-      if ord = None then
-        (list_delete_arr ls fml;
-          (fml, (inds, (id,
-                (do_core_del core ls,
-                (bound, (ord, orders)))))))
-      else
-        case all_core_arr fml inds core of (ac,inds') =>
-        if ac then
-          (list_delete_arr ls fml;
-            (fml, (inds', (id,
-                  (do_core_del core ls,
-                  (bound, (ord, orders)))))))
-        else
-           raise Fail (format_failure lno ("not all constraints in core")))
+  | Checkeddelete n s pfs idopt => (
+    case Array.lookup fml None n of None =>
+      raise Fail (format_failure lno
+        "invalid core deletion ID")
+    | Some c => (
+      if lookup_1 n core = Some () then
+        (let
+          val nc = delete_1 n core in
+          case arr_from_core_arr nc fml of (ncf,ninds) =>
+          (case
+            check_red_arr lno ord obj nc ncf ninds
+              id c s pfs idopt of (nfml',(id',ninds')) =>
+              (list_delete_arr [n] fml;
+              (fml, (inds, (id',
+                  (nc, (chk, (obj, (bound, (ord, orders))))))))))
+        end)
+      else raise Fail (format_failure lno
+        "invalid core deletion ID (non-core)")
+      ))
+  | Uncheckeddelete ls => (
+    if ord = None then
+      (list_delete_arr ls fml;
+        (fml, (inds, (id, (do_core_del core ls,
+          (False,(obj,(bound, (ord, orders)))))))))
     else
-      raise Fail (format_failure lno ("not all core del ids in core"))
-    )
-    | Sstep sstep => (
+      case all_core_arr fml inds core of (ac,inds') =>
+      if ac then
+        (list_delete_arr ls fml;
+          (fml, (inds', (id, (do_core_del core ls,
+            (False, (obj, (bound, (ord, orders)))))))))
+      else
+         raise Fail (format_failure lno ("not all constraints in core")))
+  | Sstep sstep => (
     case check_sstep_arr lno sstep ord obj core fml inds id of
       (fml',(id',inds')) =>
-      (fml',(inds',(id',(core,(bound,(ord,orders)))))))
+      (fml',(inds',(id',(core,
+        (chk,(obj,(bound,(ord,orders)))))))))
   | Obj w => (
     case check_obj obj bound w (coref_arr core fml) of
       None =>
@@ -1948,9 +2378,13 @@ val check_cstep_arr = process_topdecs`
          (sorted_insert id inds,
          (id+1,
          (insert_1 id () core,
-         (Some new, (ord, orders))))))
+         (chk,(obj,(Some new, (ord, orders))))))))
       end
-    )`
+    )
+  | Changeobj fc' n1 n2 =>
+    (check_change_obj_arr lno fml core chk obj ord fc' n1 n2;
+      (fml, (inds, (id, (core, (chk,
+        (Some fc', (bound, (ord, orders)))))))))`
   |> append_prog;
 
 val NPBC_CHECK_CSTEP_TYPE_def = theorem "NPBC_CHECK_CSTEP_TYPE_def";
@@ -1970,34 +2404,36 @@ QED
 Theorem EqualityType_ord_TYPE:
   EqualityType ord_TYPE
 Proof
-  rw[ord_TYPE_def,spo_TYPE_def,constraint_TYPE_def]>>
   metis_tac[EqualityType_OPTION_TYPE,EqualityType_PAIR_TYPE,EqualityType_LIST_TYPE,EqualityType_NUM_BOOL]
 QED
 
+(* TODO: Extremely slow *)
 Theorem check_cstep_arr_spec:
-  NPBC_CHECK_CSTEP_TYPE cstep cstepv ∧
   NUM lno lnov ∧
-  BOOL chk chkv ∧
-  ord_TYPE ord ordv ∧
-  OPTION_TYPE (LIST_TYPE (PAIR_TYPE INT NUM)) obj objv ∧
-  OPTION_TYPE NUM bound boundv ∧
+  NPBC_CHECK_CSTEP_TYPE cstep cstepv ∧
   SPTREE_SPT_TYPE UNIT_TYPE core corev ∧
-  NUM id idv ∧
+  BOOL chk chkv ∧
+  obj_TYPE obj objv ∧
+  OPTION_TYPE INT bound boundv ∧
+  ord_TYPE ord ordv ∧
+  LIST_TYPE (PAIR_TYPE STRING_TYPE spo_TYPE) orders ordersv ∧
   LIST_REL (OPTION_TYPE constraint_TYPE) fmlls fmllsv ∧
   (LIST_TYPE NUM) inds indsv ∧
-  LIST_TYPE (PAIR_TYPE STRING_TYPE spo_TYPE) orders ordersv
+  NUM id idv
   ⇒
   app (p : 'ffi ffi_proj)
     ^(fetch_v "check_cstep_arr" (get_ml_prog_state()))
-    [lnov; cstepv; chkv; ordv; objv; boundv; corev;
-      fmlv; indsv; idv; ordersv]
+    [lnov; cstepv; corev; chkv; objv; boundv; ordv; ordersv;
+      fmlv; indsv; idv]
     (ARRAY fmlv fmllsv)
     (POSTve
       (λv.
         SEP_EXISTS fmlv' fmllsv'.
         ARRAY fmlv' fmllsv' *
         &(
-          case check_cstep_list cstep chk ord obj bound core fmlls inds id orders of NONE => F
+          case check_cstep_list cstep core chk obj bound
+            ord orders fmlls inds id of
+            NONE => F
           | SOME res =>
             PAIR_TYPE (λl v.
               LIST_REL (OPTION_TYPE constraint_TYPE) l fmllsv' ∧
@@ -2005,16 +2441,18 @@ Theorem check_cstep_arr_spec:
               (PAIR_TYPE (LIST_TYPE NUM)
                 (PAIR_TYPE NUM
                 (PAIR_TYPE (SPTREE_SPT_TYPE UNIT_TYPE)
-                (PAIR_TYPE (OPTION_TYPE NUM)
+                (PAIR_TYPE BOOL
+                (PAIR_TYPE obj_TYPE
+                (PAIR_TYPE (OPTION_TYPE INT)
                 (PAIR_TYPE ord_TYPE
-                  (LIST_TYPE (PAIR_TYPE STRING_TYPE spo_TYPE)))))))
+                  (LIST_TYPE (PAIR_TYPE STRING_TYPE spo_TYPE)))))))))
               res v
           ))
       (λe.
         SEP_EXISTS fmlv' fmllsv'.
         ARRAY fmlv' fmllsv' *
         & (Fail_exn e ∧
-          check_cstep_list cstep chk ord obj bound core fmlls inds id orders = NONE)))
+          check_cstep_list cstep core chk obj bound ord orders fmlls inds id = NONE)))
 Proof
   rw[]>>
   xcf "check_cstep_arr" (get_ml_prog_state ())>>
@@ -2022,104 +2460,31 @@ Proof
   Cases_on`cstep`>>fs[NPBC_CHECK_CSTEP_TYPE_def]
   >- ( (* Dom*)
     xmatch>>
-    Cases_on`ord`>>fs[ord_TYPE_def,OPTION_TYPE_def]>>xmatch
+    Cases_on`ord`>>fs[OPTION_TYPE_def]>>xmatch
     >- (
       rpt xlet_autop>>
       xraise>> xsimpl>>
       metis_tac[Fail_exn_def,ARRAY_refl])>>
-    pairarg_tac>>xlet_autop>>
-    fs[PAIR_TYPE_def]>>
-    xmatch>>
-    rpt xlet_autop>>
-    fs[spo_TYPE_def,ord_TYPE_def,constraint_TYPE_def]>>
-    rpt xlet_autop>>
-    rename1`do_dso spo _ _ _`>>
-    rename1`VECTOR_TYPE _ s _`>>
-    xlet`(POSTve
-      (λv.
-        ARRAY fmlv fmllsv *
-        &(case extract_clauses_list s fmlls (do_dso spo s p' obj) l [] of
-            NONE => F
-          | SOME res => LIST_TYPE (PAIR_TYPE (OPTION_TYPE (PAIR_TYPE (LIST_TYPE constraint_TYPE) NUM)) (LIST_TYPE NPBC_CHECK_LSTEP_TYPE)) res v))
-    (λe.
-      ARRAY fmlv fmllsv *
-      & (Fail_exn e ∧ extract_clauses_list s fmlls (do_dso spo s p' obj) l [] = NONE)))`
-    >- (
-      xapp>>xsimpl>>
-      simp[LIST_TYPE_def,constraint_TYPE_def]>>
-      metis_tac[])
+    pairarg_tac>>xlet_autop
     >- (
       xsimpl>>
-      simp[do_dso_def]>>
-      metis_tac[ARRAY_refl])>>
-    pop_assum mp_tac>>TOP_CASE_TAC>>simp[]>>
-    fs[do_dso_def]>>
-    strip_tac>>
-    rpt xlet_autop>>
-    xlet_auto>>
-    rpt xlet_autop>>
-    fs[GSYM constraint_TYPE_def]>>
-    rename1`_ (not n) vvv`>>
-    `LIST_REL (OPTION_TYPE constraint_TYPE)
-      (update_resize fmlls NONE (SOME (not n)) id)
-      (update_resize fmllsv (Conv (SOME (TypeStamp "None" 2)) [])
-              (Conv (SOME (TypeStamp "Some" 2)) [vvv]) id)` by
-      (match_mp_tac LIST_REL_update_resize>>fs[OPTION_TYPE_def,constraint_TYPE_def])>>
-    xlet_autop
-    >- (
-      xsimpl>>rw[]>>
-      metis_tac[ARRAY_refl])>>
-    pop_assum mp_tac>>
-    TOP_CASE_TAC>>fs[]>>
-    Cases_on`x'`>>simp[PAIR_TYPE_def]>>
-    strip_tac>>
+      simp[check_dom_list_def]>>
+      rw[]>>
+      qexists_tac`x'`>>qexists_tac`x''`>>xsimpl>>
+      fs[do_dom_check_def,AllCaseEqs()])>>
+    pop_assum mp_tac>>TOP_CASE_TAC>>strip_tac>>
+    PairCases_on`x'`>>fs[PAIR_TYPE_def]>>
     xmatch>>
-    rename1`do_dom_check idopt _`>>
-    Cases_on`idopt`>>
-    fs[OPTION_TYPE_def,do_dom_check_def]>>
-    xmatch
-    >- (
-      rpt xlet_autop>>
-      fs[constraint_TYPE_def]>>
-      xlet_autop>>
-      fs[GSYM constraint_TYPE_def]>>
-      xlet_autop>>
-      reverse xif>>gs[]
-      >- (
-        rpt xlet_autop>>
-        fs[red_cond_check_def]>>pairarg_tac>>fs[core_subgoals_def]>>
-        xraise>>xsimpl>>
-        fs[red_cond_check_def]>>rw[]>>
-        metis_tac[ARRAY_refl,Fail_exn_def,NOT_EVERY])>>
-      rpt xlet_autop>>
-      xlet_auto>>
-      pairarg_tac>>fs[red_cond_check_def,core_subgoals_def]>>
-      xcon>>
-      xsimpl>>rw[]>>
-      fs[PAIR_TYPE_def,OPTION_TYPE_def]>>
-      qmatch_goalsub_abbrev_tac`ARRAY _ A`>>
-      qexists_tac`A`>>xsimpl>>
-      unabbrev_all_tac>>
-      match_mp_tac LIST_REL_update_resize>>
-      fs[OPTION_TYPE_def,constraint_TYPE_def])>>
     rpt xlet_autop>>
-    reverse xif
-    >- (
-      rpt xlet_autop>>
-      xraise>>
-      xsimpl>>
-      rw[]>>fs[]>>
-      metis_tac[ARRAY_refl,NOT_EVERY,Fail_exn_def]) >>
-    rpt xlet_autop>>
+    gvs[check_dom_list_def,AllCaseEqs()]>>
     xlet_auto>>
     xcon>>xsimpl>>
-    simp[PAIR_TYPE_def]>>
+    simp[PAIR_TYPE_def,OPTION_TYPE_def]>>
     qmatch_goalsub_abbrev_tac`ARRAY _ A`>>
     qexists_tac`A`>>xsimpl>>
     unabbrev_all_tac>>
-    fs[OPTION_TYPE_def,constraint_TYPE_def]>>
     match_mp_tac LIST_REL_update_resize>>
-    fs[OPTION_TYPE_def,constraint_TYPE_def])
+    fs[OPTION_TYPE_def])
   >- ( (* LoadOrder*)
     xmatch>>
     rpt xlet_autop>>
@@ -2128,7 +2493,6 @@ Proof
       rpt xlet_autop>>
       xraise>> xsimpl>>
       metis_tac[Fail_exn_def,ARRAY_refl])>>
-    fs[spo_TYPE_def]>>
     rpt xlet_autop>>
     reverse(IF_CASES_TAC)>>gs[]>>
     xif>>asm_exists_tac>>simp[]
@@ -2138,11 +2502,11 @@ Proof
       metis_tac[Fail_exn_def,ARRAY_refl])>>
     rpt xlet_autop>>
     xcon>>xsimpl>>
-    simp[PAIR_TYPE_def,ord_TYPE_def,OPTION_TYPE_def,spo_TYPE_def]>>
+    simp[PAIR_TYPE_def,OPTION_TYPE_def]>>
     metis_tac[ARRAY_refl])
   >- ( (* UnloadOrder *)
     xmatch>>
-    Cases_on`ord`>>fs[OPTION_TYPE_def,ord_TYPE_def]>>
+    Cases_on`ord`>>fs[OPTION_TYPE_def]>>
     xmatch
     >- (
       rpt xlet_autop>>
@@ -2150,7 +2514,7 @@ Proof
       metis_tac[Fail_exn_def,ARRAY_refl])>>
     rpt xlet_autop>>
     xcon>>xsimpl>>
-    fs[PAIR_TYPE_def,ord_TYPE_def,OPTION_TYPE_def,spo_TYPE_def]>>
+    fs[PAIR_TYPE_def,OPTION_TYPE_def]>>
     metis_tac[ARRAY_refl])
   >- ( (* StoreOrder *)
     xmatch>>
@@ -2160,7 +2524,7 @@ Proof
     >- (
       rpt xlet_autop>>
       xcon>>xsimpl>>
-      fs[PAIR_TYPE_def,ord_TYPE_def,OPTION_TYPE_def,spo_TYPE_def,LIST_TYPE_def,constraint_TYPE_def,check_storeorder_def]>>
+      fs[PAIR_TYPE_def,OPTION_TYPE_def,LIST_TYPE_def,check_storeorder_def]>>
       metis_tac[ARRAY_refl])>>
     rpt xlet_autop>>
     xraise >> xsimpl>>
@@ -2175,7 +2539,7 @@ Proof
         metis_tac[NOT_EXISTS,NOT_EVERY]>>
       rpt xlet_autop>>
       xcon>> xsimpl>>
-      fs[PAIR_TYPE_def,ord_TYPE_def,OPTION_TYPE_def,spo_TYPE_def,LIST_TYPE_def,constraint_TYPE_def,do_transfer_def]>>
+      fs[PAIR_TYPE_def,OPTION_TYPE_def,LIST_TYPE_def,do_transfer_def]>>
       metis_tac[ARRAY_refl,NOT_EXISTS,NOT_EVERY])>>
     rw[]>>
     rpt xlet_autop>>
@@ -2184,23 +2548,86 @@ Proof
     metis_tac[ARRAY_refl])
   >- ( (* CheckedDelete*)
     xmatch>>
-    xlet_autop>>
-    reverse(xif>>fs[all_core_every_def])
+    rpt xlet_autop>>
+    xlet_auto>>
+    rename1`cv = any_el n _ _`>>
+    `OPTION_TYPE constraint_TYPE (any_el n fmlls NONE) cv` by (
+      rw[any_el_ALT]>>
+      fs[LIST_REL_EL_EQN,OPTION_TYPE_def])>>
+    qpat_x_assum`cv = _` (assume_tac o SYM)>>
+    Cases_on`any_el n fmlls NONE`>>
+    fs[OPTION_TYPE_def]>>xmatch
     >- (
       rpt xlet_autop>>
-      qpat_x_assum`EXISTS _ _` mp_tac>>
-      REWRITE_TAC [GSYM NOT_EVERY]>>
-      strip_tac>>
-      simp[]>>
-      xraise >> xsimpl>>
+      xraise>>xsimpl>>
       fs[Fail_exn_def]>>
       metis_tac[ARRAY_refl])>>
-    xif
+    rpt xlet_autop>>
+    xlet`POSTv v. ARRAY fmlv fmllsv * &BOOL (lookup n core = SOME()) v`
+    >- (
+      xapp_spec (mlbasicsProgTheory.eq_v_thm |> INST_TYPE [alpha |-> ``:unit option``])>>
+      xsimpl>>
+      first_x_assum (irule_at Any)>>
+      qexists_tac`SOME ()`>>simp[OPTION_TYPE_def,BOOL_def]>>
+      metis_tac[EqualityType_OPTION_TYPE,EqualityType_NUM_BOOL])>>
+    reverse xif
     >- (
       rpt xlet_autop>>
-      xraise >> xsimpl>>
+      xraise>>xsimpl>>
       fs[Fail_exn_def]>>
       metis_tac[ARRAY_refl])>>
+    rpt xlet_autop>>
+    xlet_auto
+    >- (
+      xsimpl>>
+      metis_tac[ARRAY_refl])>>
+    pairarg_tac>>fs[PAIR_TYPE_def]>>
+    xmatch>>
+    xlet`(POSTve (λvv.
+       SEP_EXISTS fmlv' fmllsv'.
+         ARRAY fmlv fmllsv *
+         &case
+           check_red_list ord obj (delete n core) ncf ninds id x v l o'
+         of
+           NONE => F
+         | SOME res =>
+           PAIR_TYPE
+             (λl v.
+                  LIST_REL (OPTION_TYPE constraint_TYPE) l fmllsv' ∧
+                  v = fmlv') (PAIR_TYPE NUM (LIST_TYPE NUM)) res vv)
+    (λe.
+         ARRAY fmlv fmllsv *
+         &(Fail_exn e ∧
+          check_red_list ord obj (delete n core) ncf ninds id x v l o' = NONE)))`
+    >- (
+      xapp>>
+      simp[PULL_EXISTS]>>
+      rpt(asm_exists_tac>>simp[])>>
+      xsimpl>>
+      metis_tac[ARRAY_refl])
+    >- (
+      xsimpl>>
+      metis_tac[ARRAY_refl])>>
+    pop_assum mp_tac>>
+    TOP_CASE_TAC>>PairCases_on`x'`>>fs[PAIR_TYPE_def]>>
+    rw[]>>
+    qpat_x_assum`_ fmllsv'` kall_tac>>
+    qpat_x_assum`_ nfmllsv` kall_tac>>
+    xmatch>>
+    rpt xlet_autop>>
+    xlet`POSTv resv.
+         &UNIT_TYPE () resv *
+         SEP_EXISTS fmllsv'.
+           ARRAY fmlv fmllsv' *
+           &LIST_REL (OPTION_TYPE constraint_TYPE)
+             (list_delete_list [n] fmlls) fmllsv'`
+    >- (
+      xapp>>
+      simp[LIST_TYPE_def])>>
+    rpt xlet_autop>>
+    xcon>>xsimpl)
+  >- ( (* Uncheckeddelete *)
+    xmatch>>
     rpt xlet_autop>>
     xlet`POSTv v. ARRAY fmlv fmllsv * &(BOOL (ord = NONE) v)`
     >- (
@@ -2208,15 +2635,14 @@ Proof
       xsimpl>>
       first_x_assum (irule_at Any)>>
       qexists_tac`NONE`>>simp[OPTION_TYPE_def]>>
-      rw[] >- metis_tac[EqualityType_ord_TYPE]>>
-      EVAL_TAC)>>
+      metis_tac[EqualityType_ord_TYPE])>>
     xif
     >- (
       rpt xlet_autop>>
       xcon>>xsimpl>>
       simp[PAIR_TYPE_def]>>
-      fs[do_core_del_def,ord_TYPE_def,ord_TYPE_def]>>
-      metis_tac[ARRAY_refl])>>
+      fs[do_core_del_def]>>
+      xsimpl)>>
     rpt xlet_autop>>
     pairarg_tac>>fs[PAIR_TYPE_def]>>
     xmatch>>
@@ -2225,12 +2651,11 @@ Proof
       rpt xlet_autop>>
       xcon>>xsimpl>>
       simp[PAIR_TYPE_def]>>
-      fs[do_core_del_def,ord_TYPE_def,ord_TYPE_def]>>
-      metis_tac[ARRAY_refl])>>
+      fs[do_core_del_def]>>
+      xsimpl)>>
     rpt xlet_autop>>
     xraise>>xsimpl>>
-    metis_tac[Fail_exn_def,ARRAY_refl]
-  )
+    metis_tac[Fail_exn_def,ARRAY_refl])
   >- ( (* Sstep *)
     xmatch>>
     xlet_autop
@@ -2245,8 +2670,6 @@ Proof
     xcon>>xsimpl)
   >- ( (* Obj *)
     xmatch>>
-    xlet_autop>>
-    fs[constraint_TYPE_def]>>
     rpt xlet_autop>>
     Cases_on`check_obj obj bound s (coref_list core fmlls)`>>
     fs[OPTION_TYPE_def]>>xmatch
@@ -2256,7 +2679,6 @@ Proof
       fs[Fail_exn_def]>>
       metis_tac[ARRAY_refl])>>
     rpt xlet_autop>>
-    fs[constraint_TYPE_def]>>
     xlet_auto>>
     xcon>>xsimpl>>
     simp[PAIR_TYPE_def,OPTION_TYPE_def]>>
@@ -2264,7 +2686,17 @@ Proof
     qexists_tac`A`>>xsimpl>>
     unabbrev_all_tac>>
     match_mp_tac LIST_REL_update_resize>>
-    fs[OPTION_TYPE_def,constraint_TYPE_def])
+    fs[OPTION_TYPE_def])
+  >- ( (* ChangeObj *)
+    xmatch>>
+    rpt xlet_autop
+    >- (
+      xsimpl>>
+      simp[Fail_exn_def]>>
+      metis_tac[ARRAY_refl,Fail_exn_def])>>
+    xcon>>xsimpl>>
+    simp[PAIR_TYPE_def,OPTION_TYPE_def]>>
+    metis_tac[ARRAY_refl])
 QED
 
 val _ = export_theory();
